compiler/proof_vec/new_test_proof.ec
@@ -11,7 +11,7 @@ hint simplify (pack_unpack_4u32, unpack_pack_4u32)@0.
 hint simplify (VPAND_128_32, VPOR_128_32, VPXOR_128_32)@0.
 
 axiom rol32_xor (x:W32.t) i : 0 <= i < 32 => 
- (x86_ROL_32 x ((of_int i)%W8)).`3  = (x `<<` (W8.of_int i)) `^` (x `>>` (W8.of_int (32 - i))).
+ (x86_ROL_32 x ((of_uint i)%W8)).`3  = (x `<<` (W8.of_uint i)) `^` (x `>>` (W8.of_uint (32 - i))).
 
 equiv rotate_ref_ref1 : Gimli_ref.M.rotate ~ Gimli_ref1.M.rotate : ={x,bits} /\ 0 <= bits{1} < 32 ==> ={res}.
 proof.
@@ -43,8 +43,8 @@ proof.
 qed.
 
 axiom rotate24E w :
-    x86_VPSHUFB_128  w (W128.of_int 16028905388486802350658220295983399425)
-  = x86_VPSLL_4u32 w (W8.of_int 24) `^` x86_VPSRL_4u32 w (W8.of_int 8).
+    x86_VPSHUFB_128  w (W128.of_uint 16028905388486802350658220295983399425)
+  = x86_VPSLL_4u32 w (W8.of_uint 24) `^` x86_VPSRL_4u32 w (W8.of_uint 8).
 
 hint simplify rotate24E.
 
